src/axiomatic/PFtoA4OBR.v
@@ -62,7 +62,7 @@ Lemma sim_traces_sim_th'_ob_read
     (RL: lastn (S n) rl = r2 :: r1 :: rl')
     (COV: lastn (S n) covl = cov2 :: cov1 :: covl')
     (VEXT: lastn (S n) vextl = vext2 :: vext1 :: vextl')
-    (SIM_TH': sim_th' tid ex (v_gen vexts) eu1 aeu1),
+    (SIM_TH': sim_th' tid m.(Machine.mem) ex (v_gen vexts) eu1 aeu1),
     sim_ob_read tid ex (v_gen vexts) eu2 aeu2.
 Proof.
   i. rename SIM_TH' into L.
@@ -108,7 +108,11 @@ Proof.
   rewrite EX2.(XVEXT); s; cycle 1.
   { rewrite List.app_length. s. clear. lia. }
   rewrite X.
-  inv STEP0. ss. subst. inv LOCAL0; inv EVENT. inv STEP0. ss.
+  inv STEP0. ss. subst. inv LOCAL0; inv EVENT.
+  exploit sim_trace_sim_th; try exact TRACE; eauto. intro SIM_TH.
+  destruct SIM_TH.(EU_WF).
+  specialize (Local.read_spec LOCAL0 STEP0). i. des.
+  clear STATE2 LOCAL0. inv STEP0. ss.
   exploit EX2.(LABELS); eauto; ss.
   { rewrite List.app_length. s. clear. lia. }
   i.
@@ -117,13 +121,8 @@ Proof.
     assert (v_gen vexts eid1 = ts).
     { inv H. destruct eid1 as [tid1 eid1]. inv H2. ss.
       generalize H1. intro Y. rewrite RF in Y. inv Y. ss.
-      assert (r (length (ALocal.labels alc1)) =
-              (fun eid : nat =>
-                 if eid =? length (ALocal.labels alc1)
-                 then Some (ValA.val vloc, fun_add (ValA.val vloc) ts (Local.coh lc1) (ValA.val vloc))
-                 else r1 eid) (length (ALocal.labels alc1))).
-      { eapply EX2.(XR); eauto. s. rewrite List.app_length. s. clear. lia. }
-      rewrite H in R. clear H.
+      erewrite EX2.(XR) in R; eauto; cycle 1.
+      { s. rewrite List.app_length. s. clear. lia. }
       destruct (length (ALocal.labels alc1) =? length (ALocal.labels alc1)); ss.
       rewrite fun_add_spec in R.
       destruct (equiv_dec (ValA.val vloc) (ValA.val vloc)); cycle 1.
@@ -133,7 +132,14 @@ Proof.
       exploit sim_trace_last; try exact REL0. i. des. simplify.
       exploit sim_trace_sim_th; try exact REL0; eauto. intro L1.
       exploit L1.(WPROP3); eauto. i. des.
-      unfold v_gen. ss. rewrite <- H7. ss. }
+      unfold v_gen. ss. rewrite <- H7.
+      exploit Memory.latest_latest_ts; try exact COH; eauto. i.
+      rewrite fun_add_spec in x8. revert x8. condtac; ss. i.
+      unfold FwdItem.read_view in *. revert x4. condtac.
+      - i.
+      exploit sim_trace_sim_th; try exact TRACE; eauto. intro L2.
+      destruct L2.(EU_WF). destruct LOCAL0. ss.
+    }
     subst.
     rewrite <- join_r. unfold FwdItem.read_view. condtac; ss.
     destruct (equiv_dec (FwdItem.ts (Local.fwdbank lc1 (ValA.val vloc))) (v_gen vexts eid1)); ss. inv e.
